chore: integrate operators into KLR.Core
This change integrates the operators from KLR.KLR into KLR.Core in preparation
for tracing from NKI.Basic. The definition of TensorRef wsa extended to include
the abstract TensorSBuf (previously TensorName) types as a variant.

KLR/Core/Basic.lean
@@ -3,7 +3,7 @@ Copyright (c) 2024 Amazon.com, Inc. or its affiliates. All Rights Reserved.
 Released under Apache 2.0 license as described in the file LICENSE.
 Authors: Paul Govereau, Sean McLaughlin
 -/
-import Init.Data.Int.Basic
+import KLR.Core.Tensor
 import KLR.Core.Operators
 import KLR.Serde.Attr
 import KLR.Serde.Elab
@@ -21,6 +21,9 @@ open Lean (FromJson ToJson)
 open Serde (FromCBOR ToCBOR)
 open Util (FromSexp ToSexp)
 
+export Lean (Name)
+deriving instance Ord for Name
+
 /-
 A source position records the location of a statement in the original program.
 -/
@@ -34,316 +37,20 @@ structure Pos where
   deriving BEq, FromCBOR, FromJson, FromSexp, Repr, ToCBOR, ToJson, ToSexp
 
 /-
-A tensor shape is a list of the sizes of each dimension of the tensor. By
-convention, the first dimension is always the "partition" dimension, and the
-remaining dimensions are "free" dimensions. When laid out in memory, the
-partition dimension will correspond to the memory partition.
--/
-
-structure Shape where
-  parDim : Nat
-  freeDims : List Nat
-  deriving Repr, BEq, Inhabited
-
-def Shape.toList (shape : Shape) : List Nat :=
-  shape.parDim :: shape.freeDims
-
-def Shape.fromList : List Nat -> Err Shape
-  | [] => throw "invalid shape"
-  | p :: f => return ⟨ p, f ⟩
-
-instance : ToString Shape where
-  toString shape := toString shape.toList
-
-def Shape.freeElements (shape : Shape) : Nat :=
-  shape.freeDims.foldl (. * .) 1
-
-/-
-An Address represents a region of memory. Each address has a memory type, and
-the starting location and size of the memory region. The memory regions are
-always two-dimensional and the start and size are expressed in bytes. The
-starting location can be omitted to have the compiler choose this for you.
-
-An address may have a parent, in which case the start is relative to the
-parent's start location. This allows the user to declare a memory region with
-no start address, but containing subregions with specific relative positions.
-
-The Address structure is represented as a "pointer" term during tracing.
--/
-
-structure Address where
-  memory : Memory
-  size : Nat × Nat
-  partitionOffset : Option Nat := none
-  freeOffset : Option Nat := none
-  parent : Option Address := none
-  deriving Repr, BEq
-
-namespace Address
-
-def defaultSize (shape : Shape) (dtype : Dtype) : (Nat × Nat) :=
-  (shape.parDim, shape.freeElements * dtype.size)
-
-def withDefaultSize (addr : Address) (shape : Shape) (dtype : Dtype) : Address :=
-  { addr with size := defaultSize shape dtype }
-
-end Address
-
-/--
-TensorName represents a tensor in memory at runtime. Each runtime tensor has a
-dtype, shape, and address. The address size must be large enough to hold the
-tensor.
--/
-
-structure TensorName where
-  name    : String
-  dtype   : Dtype
-  shape   : Shape
-  address : Address
-  parWF   : shape.parDim <= address.size.fst
-  freeWF  : shape.freeElements * dtype.size <= address.size.snd
-  deriving Repr
-
-namespace TensorName
-
-def make (name : String)
-         (dtype : Dtype)
-         (shape : Shape)
-         (addr : Option Address) : Err TensorName := do
-  let addr := addr.getD { memory := .sbuf, size := Address.defaultSize shape dtype }
-  if parWF: shape.parDim <= addr.size.fst then
-    if freeWF: shape.freeElements * dtype.size <= addr.size.snd then
-      return ⟨ name, dtype, shape, addr, parWF, freeWF ⟩
-  throw "Invalid tensor"
-
-def withShape (name : TensorName) (shape : Shape) : Err TensorName :=
-  make name.name name.dtype shape (name.address.withDefaultSize shape name.dtype)
-
-instance : BEq TensorName where
-  beq l r := l.name == r.name &&
-             l.dtype == r.dtype &&
-             l.shape == r.shape &&
-             l.address == r.address
-
-end TensorName
-
-/--
-Basic indexing elements: integers and slices.
-These are used for basic indexing, such as:
-  t[1, 2]
-  t[0:10, :]
-  t[5, 0:10:2]
-
-The tracing process will generate Indexes relative to a given shape,
-and therefore we do not have `None` or `...` as possibilities.
--/
-structure Slice where
-  l : Nat
-  u : Nat
-  step : Int
-  wf : step ≠ 0
-deriving Repr
-
-namespace Slice
-
-def make (l u : Nat) (step : Int) : Err Slice :=
-  if H : step == 0 then throw "step can't be 0"
-  else return Slice.mk l u step (by simp_all)
-
-instance : Inhabited Slice where
-  default := Slice.mk 0 1 1 (by omega)
-
-def make! (l u : Nat) (step : Int) : Slice := get! $  make l u step
-
-instance : BEq Slice where
-  beq s1 s2 := s1.l == s2.l && s1.u == s2.u && s1.step == s2.step
-
-def size (slice : Slice) : Nat :=
-  let step := slice.step
-    if step < 0 then (slice.l - slice.u) / step.natAbs
-    else natDivCeil (slice.u - slice.l) step.toNat
-
-#guard (make! 0 10 1).size == 10
-#guard (make! 10 0 (-1)).size == 10
-#guard (make! 0 10 (-1)).size == 0
-#guard (make! 10 0 1).size == 0
-
-end Slice
-
-inductive Index where
-  | coord (e : Nat)
-  | slice (slice : Slice)
-  deriving Repr, BEq
-
--- Compute the number of elements an index represents
-def Index.size : Index -> Nat
- | .coord _ => 1
- | .slice s => s.size
-
-/--
-Complete Basic Indexing expression
-
-The number of indexes must match the dimension of the tensor.
--/
-
-structure AccessBasic where
-  tensor : TensorName
-  indexes : List Index
-  lenWF : tensor.shape.freeDims.length + 1 = indexes.length
-  deriving Repr
-
-instance : BEq AccessBasic where
-  beq l r := l.tensor == r.tensor && l.indexes == r.indexes
-
-def AccessBasic.make (t : TensorName) (i : List Index) : Err AccessBasic := do
-  if lenWF : t.shape.freeDims.length + 1 = i.length then
-    return ⟨ t, i, lenWF ⟩
-  throw "invalid basic access"
-
-def AccessBasic.shape (a : AccessBasic) : Err Shape :=
-  if let p::l := a.indexes then
-    .ok ⟨ p.size, l.map Index.size ⟩
-  else .error "invalid access"
-
-theorem AccessBasic.shape.noFail :
-  forall (a : AccessBasic), AccessBasic.shape a ≠ Except.error s := by
-  intro a
-  unfold AccessBasic.shape
-  let { tensor, indexes, lenWF : AccessBasic } := a
-  induction indexes <;> simp ; trivial
-  done
-
-/--
-Access pattern elements.
-
-These are used for HW-native indexing which consists of an offset and a list of
-access pattern pairs. Each pair specifies a step size and the number of steps
-to take. The first changes the slowest, and the last pair changes the fastest.
-For example, in the list of pairs:
-
-  [ (3,2), (1,3) ]
-
-the first pair will produce the values 0,3 and the second pair will produce the
-values 0,1,2. Added together, the pairs produce the values:
-
-  0, 1, 2, 3, 4, 5.
-
-which is equivalent to the basic index [0:2,0:3] for a standard tensor layout.
--/
-structure APPair where
-  step : Int := 1
-  num : Nat := 1
-  deriving Repr, BEq
-
-/--
-Complete access patterns
-
-A complete access pattern has a list of APPairs, a number of partitions, and an
-offset. In NKI, the first access pattern pair corresponds to the partition
-dimension, and the step size of this first pair must be one. So, in the
-complete access pattern, we only store the `num` field of the first pair. The
-offset field allows for an arbitrary offset to be applied to each partition.
-
-Put together, a complete access pattern would be written as:
-
-  t[[ offset, (1, parNum), (step1,num1), (step2,num2), ... ]]
-
-With a meaning of:
-
-  forall p < parNum, x < num1, y < num2, ...
-    offset + p + x * step1 + y * step2 + ...
-
-The elements generated above are multiplied by the dtype size of the tensor to
-get the final memory addresses.
--/
-
-structure AccessPattern where
-  tensor : TensorName
-  parNum : Nat
-  freePattern : List APPair
-  offset : Nat := 0
-  deriving Repr, BEq
-
-namespace AccessPattern
-
-def shape (ap : AccessPattern) : Shape :=
-  .mk ap.parNum $ ap.freePattern.map fun pair => pair.num
-
-private def withNoParents (ap : AccessPattern) (f : AccessPattern -> a) : Err a :=
-  if ap.tensor.address.parent.isSome
-    then throw "Please compile away the parent indirections"
-  else return f ap
-
--- Partitions are not counted in bytes or elements; I'll call them logical "rows".
-def partitionRowOffset (ap : AccessPattern) : Err Nat := ap.withNoParents fun ap =>
-  ap.tensor.address.partitionOffset.getD 0
-
-private def freeByteOffset' (ap : AccessPattern) := ap.tensor.address.freeOffset.getD 0 + ap.offset
-
-def freeByteOffset (ap : AccessPattern) : Err Nat := ap.withNoParents freeByteOffset'
-
--- We can't find documentation that the free offset must be aligned by dtype size, but we think
--- it's probably the case. It certainly makes calculating indexes easier so we're going with it
--- for now.
-def freeElementOffset (ap : AccessPattern) : Err Nat := ap.withNoParents fun ap =>
-  ap.freeByteOffset' / ap.tensor.dtype.size
-
-end AccessPattern
-
--- Tensor access: whole tensor (simple), basic indexing, or access pattern
--- TODO: add advanced indexing (tensor indirect) inductive Access where
-
-inductive Access where
-  | simple  : TensorName -> Access
-  | basic   : AccessBasic -> Access
-  | pattern : AccessPattern -> Access
-  deriving Repr, BEq
-
-def Access.mkBasic (t : TensorName) (i : List Index) : Err Access :=
-  return .basic (<- AccessBasic.make t i)
-
-def Access.tensor : Access -> TensorName
-  | simple tensor | basic {tensor, ..} | pattern {tensor, ..} => tensor
-
-def Access.shape : Access -> Err Shape
-  | .simple t => return t.shape
-  | .basic b => b.shape
-  | .pattern ap => return ap.shape
-
-theorem Access.shape.noFail :
-  forall (a : Access), Access.shape a ≠ Except.error s := by
-  unfold Access.shape pure
-  unfold Applicative.toPure
-  unfold Monad.toApplicative
-  unfold Except.instMonad Except.pure
-  intro a
-  induction a <;> simp
-  apply AccessBasic.shape.noFail
-  done
-
--- We could make a pure variant of shape, but proofs about this
--- function may be difficult due to the dependent matching
-def Access.shapePure (a : Access) : Shape :=
-  match m:a.shape with
-  | .ok x => x
-  | .error _ =>
-     have h : False := by apply (shape.noFail a); trivial
-     nomatch h
-
-/-
 Fully reduced values
 
 While it may seem strange, an `Access` is really a value. It succinctly
 describes an (admittedly complex) set of physical memory locations. However,
 we only lookup or set the bits in those locations when applied to an operator.
 -/
+@[serde tag = 101]
 inductive Value where
   | var (x : String)
   | bool (value : Bool)
   | int (value : Int)
   | float (value : Float)
   | access (a : Access)
-  deriving Repr, BEq
+  deriving BEq, FromCBOR, FromJson, FromSexp, Repr, ToCBOR, ToJson, ToSexp
 
 /--
 Expressions are trivial right now, waiting on dynamic loops.
@@ -351,32 +58,45 @@ Expressions are trivial right now, waiting on dynamic loops.
 The call expression would only appear in a KLR program if the tracer
 encountered an unknown function.
 -/
+@[serde tag = 102]
+structure Keyword where
+  name : String
+  value : Value
+  deriving BEq, FromCBOR, FromJson, FromSexp, Repr, ToCBOR, ToJson, ToSexp
+
+@[serde tag = 103]
 inductive Expr where
   | value (v : Value)
-  | call (f : String) (args : List Value) (kwargs : List (String × Value))
-  deriving Repr, BEq
+  | call (f : String) (args : List Value) (kwargs : List Keyword)
+  deriving BEq, FromCBOR, FromJson, FromSexp, Repr, ToCBOR, ToJson, ToSexp
 
+@[serde tag = 104]
 inductive Stmt where
   | ret (v : Value)
   | assign (x : String) (e : Expr)
   | store (dst : Access) (op : Operator) (args : List Value)
-  deriving Repr
+  --| operator (op : Operator)
+  deriving BEq, FromCBOR, FromJson, FromSexp, Repr, ToCBOR, ToJson, ToSexp
 
+@[serde tag = 105]
 structure Kernel where
   name : String
-  inputs : List TensorName
-  outputs : List TensorName
+  inputs : List TensorArg
+  outputs : List TensorArg
   body : List Stmt
-  deriving Repr
+  deriving BEq, FromCBOR, FromJson, FromSexp, Repr, ToCBOR, ToJson, ToSexp
 
 -- Utilities
 
 class Tensors (a : Type) where
-  tensors : a -> List TensorName
+  tensors : a -> List TensorSram
 export Tensors (tensors)
 
-instance : Tensors TensorName where
+instance : Tensors TensorSram where
   tensors tn := [tn]
+
+instance : Tensors TensorArg where
+  tensors | .sram t => [t] | _ => []
 
 -- TODO: not efficient
 instance [inst : Tensors a] : Tensors (List a) where
@@ -393,7 +113,7 @@ instance : Tensors Value where
 instance : Tensors Expr where
   tensors
   | .value v => tensors v
-  | .call _ args kwargs => tensors (args ++ kwargs.map Prod.snd)
+  | .call _ args kwargs => tensors (args ++ kwargs.map fun kw => kw.value)
 
 instance : Tensors Stmt where
   tensors
@@ -401,6 +121,6 @@ instance : Tensors Stmt where
   | .assign _ e => tensors e
   | .store dst _ vs => tensors (tensors dst :: vs.map tensors)
 
-def Kernel.internal (k : Kernel) : List TensorName :=
+def Kernel.internal (k : Kernel) : List TensorSram :=
   let ts := (k.body.map tensors).flatten.eraseDups
-  (ts.removeAll k.inputs).removeAll k.outputs
+  (ts.removeAll (tensors k.inputs)).removeAll (tensors k.outputs)
