KLR.lean
@@ -4,7 +4,8 @@ Released under Apache 2.0 license as described in the file LICENSE.
 Authors: Paul Govereau, Sean McLaughlin
 -/
 import KLR.Core
-import KLR.Eval
+-- TODO: fix eval after big change to Core Operators
+--import KLR.Eval
 import KLR.File
 import KLR.NKI
 import KLR.Python
