KLR/Core/Operators.lean
@@ -1,73 +1,62 @@
 /-
 Copyright (c) 2025 Amazon.com, Inc. or its affiliates. All Rights Reserved.
 Released under Apache 2.0 license as described in the file LICENSE.
-Authors: Paul Govereau, Sean McLaughlin
+Authors: Paul Biberstein, Paul Govereau, Pavel Potapov, Sean McLaughlin, Markus De Medeiros
 -/
+import KLR.Core.Tensor
+import KLR.Serde.Attr
+import KLR.Serde.Elab
+import KLR.Util
+import Lean
 
 /-
 # Definition of operators
 
-Operators can appear in a call node, and can be thought of as functions that
-take arguments and return results. However, an operator may have several
-variations, and these variations show up as parameters within the operator and
-not as arguments of the call node. A typical example is:
-
-  .store t [] (.call (.operator (.tensorScalar ts)) [a,b] [])
-
-where `ts` contains the tensor scalar parameters:
-
-  let ts := TensorScalar { op0 := .add, ..}
-  let ts := TensorScalar { op0 := .multiply, op1 := add, ..}
-
-The choice of argument or parameter may seem arbitrary; these definitions
-follow the hardware ISA as close as possible.
+These definitions follow the hardware ISA as close as possible.
 -/
 namespace KLR.Core
+open Lean (FromJson ToJson)
+open Serde (FromCBOR ToCBOR)
+open Util (FromSexp ToSexp)
 
 -- Compute Engines
+@[serde tag = 130]
 inductive Engine where
   | unassigned
   | act | dma | dve | pe | pool | sp
-  deriving BEq, Repr
+  deriving BEq, FromCBOR, FromJson, FromSexp, Repr, ToCBOR, ToJson, ToSexp
 
--- Memory types
-inductive Memory where
-  | hbm | sbuf | pmem | reg
-  deriving Repr, BEq
+@[serde tag = 131]
+inductive Immediate where
+  | register (reg : Reg)
+  | pointer -- TODO
+  | int (i : Int32)
+  | float (f : Float32)
+  deriving BEq, FromCBOR, FromJson, FromSexp, Repr, ToCBOR, ToJson, ToSexp
+
+@[serde tag = 132]
+inductive ActivationImm where
+  | register (reg : Reg)
+  | pointer -- : TODO
+  | float (f : Float32)
+  deriving BEq, FromCBOR, FromJson, FromSexp, Repr, ToCBOR, ToJson, ToSexp
 
 /-
-Tensor element types supported by HW and available from NKI.
-
-The HW always performs operations on 32-bit types. However, when reading from
-or writing to memory, automatic conversion to and from the following types is
-supported.
+Used for Iota and AffineSelect, represents something similar to an
+TensorView but that is only used to generate data, not to index. Much like
+LEA in x86.
 -/
-inductive Dtype where
-  | bfloat16
-  | float8e3 | float8e4 | float8e5
-  | float16 | float32 | float32r
-  | int8 | int16 | int64 | int32
-  | uint8 | uint16 | uint32 | uint64
-  with
-    @[computed_field]
-    size : Dtype -> Nat
-    | .uint8 | .int8 | .float8e3 | .float8e4 | .float8e5 => 1
-    | .uint16 | .int16 | .bfloat16 | .float16 => 2
-    | .uint32 | .int32 | .float32 | .float32r => 4
-    | .uint64 | .int64 => 8
-    @[computed_field]
-    isInt : Dtype -> Bool
-    | .int8 | .int16 | .int64 | .int32
-    | .uint8 | .uint16 | .uint32 | .uint64 => true
-    | _ => false
-
-  deriving Repr, BEq
+@[serde tag = 133]
+structure DataPattern where
+  offset  : Nat
+  pattern  : List APPair
+  deriving BEq, FromCBOR, FromJson, FromSexp, Repr, ToCBOR, ToJson, ToSexp
 
 /-
 ALU operations supported by the HW
 Only used by: TensorScalar, TensorScalarPtr, TensorReduce, TensorTensor
 -/
-
+@[serde tag = 134]
 inductive AluOp where
   | abs
   | add
@@ -98,7 +87,7 @@ inductive AluOp where
   | pow
   | rsqrt
   | subtract
-  deriving BEq, Repr
+  deriving BEq, FromCBOR, FromJson, FromSexp, Repr, ToCBOR, ToJson, ToSexp
 
 namespace AluOp
 
@@ -118,58 +107,462 @@ def isArith : AluOp -> Bool
   | .bypass => true
   | op => not op.isBitwise
 
+-- TODO: Why do we need both Bool and Prop?
+-- TODO: can this just be isArith x == true ?
+def IsArith : AluOp → Prop
+| .abs | .add | .average | .bypass | .divide | .is_equal | .is_ge | .is_gt | .is_le | .is_lt | .max | .min | .mod | .mult | .not_equal | .pow | .rsqrt | .subtract => True
+| _ => False
+
+/-- The ALUOps for a TensorReduceArithOp -/
+def IsTensorReduceArithOp : AluOp → Prop
+| abs | add | average | bypass | is_equal | is_ge | is_gt | is_le | is_lt | max | min | mult | not_equal | subtract => True
+| _ => False
+
+/-- The ALUOps for a TensorReduceBitvecOp -/
+def IsTensorReduceBitwiseOp : AluOp → Prop
+| arith_shift_left | arith_shift_right | bitwise_and | bitwise_or | bitwise_xor | logical_and | logical_or | logical_shift_left | logical_shift_right | logical_xor => True
+| _ => False
+
 instance : ToString AluOp where
   toString op := reprStr op
 
 end AluOp
 
--- TODO: should these be Int32 and Float32?
--- At the python level: no, after tracing: yes.
--- Perhaps FromNKI can check for overflow and raise an error?
-inductive Const where
-  | int (i : Int)
-  | float (f : Float)
-  deriving BEq, Repr
+/- Whether the dropout rate is how many values should be dropped or how many
+values should be kept -/
+@[serde tag = 135]
+inductive DropoutThresholdType
+  | DropRate
+  | KeepRate
+  deriving BEq, FromCBOR, FromJson, FromSexp, Repr, ToCBOR, ToJson, ToSexp
 
-namespace Const
+/- Control how data is accumulated at destination locations -/
+@[serde tag = 136]
+inductive AccumCmd where
+  | Idle
+  | Zero
+  | Accumulate
+  | ZeroAccumulate
+  | LoadAccumulate
+  deriving BEq, FromCBOR, FromJson, FromSexp, Repr, ToCBOR, ToJson, ToSexp
 
-def isInt : Const -> Bool
-  | .int _ => true | _ => false
+@[serde tag = 137]
+inductive ActivationFunc where
+  | abs
+  | arctan
+  | copy
+  | erf
+  | erf_dx
+  | exp
+  | gelu
+  | gelu_apprx_tanh
+  | gelu_dx
+  | log
+  | mish
+  | reciprocal
+  | relu
+  | rsqrt
+  | sigmoid
+  | sign
+  | silu
+  | silu_dx
+  | sin
+  | softplus
+  | sqrt
+  | square
+  | tanh
+  deriving BEq, FromCBOR, FromJson, FromSexp, Repr, ToCBOR, ToJson, ToSexp
 
-def isFloat : Const -> Bool
-  | .float _ => true | _ => false
+/- The comparator for an affine select -/
+@[serde tag = 138]
+inductive AffineSelectCmp where
+  | GreaterThan
+  | GreaterThanEq
+  | Eq
+  | NotEq
+  deriving BEq, FromCBOR, FromJson, FromSexp, Repr, ToCBOR, ToJson, ToSexp
 
-instance : ToString Const where
-  toString
-  | .int i => toString i
-  | .float f => toString f
+/- RMW ops for DMA -/
+@[serde tag = 139]
+inductive DgeComputeOp where
+  | none
+  | add
+  deriving BEq, FromCBOR, FromJson, FromSexp, Repr, ToCBOR, ToJson, ToSexp
 
-end Const
+/- The DMA bounds check flag can either be an immediate or in a register -/
+@[serde tag = 140]
+inductive DmaBounds where
+  | disable
+  | enable
+  | reg (reg : Reg)
+  deriving BEq, FromCBOR, FromJson, FromSexp, Repr, ToCBOR, ToJson, ToSexp
 
--- Tensor-Scalar operator
--- Note: this is not supported in NKI, but it useful for testing.
-structure TensorScalar where
-  op0 : AluOp
-  const0 : Float32
-  reverse0 : Bool
-  op1 : AluOp
-  const1 : Float32
-  reverse1 : Bool
-  deriving Repr, BEq
+/- Indicates whether this is the first, middle, or last matmul
+instruction in a series of instructions that are accumulating into a region
+of psum -/
+@[serde tag = 141]
+inductive MatmulGroupElement where
+  | first
+  | middle
+  | last
+  deriving BEq, FromCBOR, FromJson, FromSexp, Repr, ToCBOR, ToJson, ToSexp
 
--- Tensor-Scalar where the scalars are loaded from memory
-structure TensorScalarAddr where
-  op0 : AluOp
-  reverse0 : Bool
-  op1 : AluOp
-  reverse1 : Bool
-  deriving Repr, BEq
+/- Whether an immediate should be written, or nothing should be written, when an index misses -/
+@[serde tag = 142]
+inductive IndexMissBehavior where
+  | imm (value : Immediate)
+  | skip
+  deriving BEq, FromCBOR, FromJson, FromSexp, Repr, ToCBOR, ToJson, ToSexp
 
--- All of the operators
+/- Which of the ops to TensorScalar should be reversed (only matters for
+non-commutative operators)-/
+@[serde tag = 143]
+inductive TensorScalarReverseOps where
+  | none
+  | first
+  | second
+  | both
+  deriving BEq, FromCBOR, FromJson, FromSexp, Repr, ToCBOR, ToJson, ToSexp
+
+/- A representation of a contiguous set of axes of a tensor -/
+@[serde tag = 144]
+inductive TensorSubDim where
+  | X
+  | XY
+  | XYZ
+  | XYZW
+  deriving BEq, FromCBOR, FromJson, FromSexp, Repr, ToCBOR, ToJson, ToSexp
+
+def TensorSubDim.IsCopySubDim : TensorSubDim → Prop
+| X => True | _ => False
+
+/- Dropout instruction -/
+@[serde tag = 145]
+structure Dropout where
+  dst           : TensorRef
+  src           : TensorRef
+  thresholdType : DropoutThresholdType
+  threshold     : Immediate
+  deriving BEq, FromCBOR, FromJson, FromSexp, Repr, ToCBOR, ToJson, ToSexp
+
+/- Activate instruction
+
+Performs the operation
+`OUT accum= activate_func( (IN * scale_value) + bias, imm )`
+-/
+@[serde tag = 146]
+structure Activate where
+  dst             : TensorRef
+  src             : TensorRef
+  accumulatorCmd  : AccumCmd
+  activationFunc  : ActivationFunc
+  scale           : Immediate
+  bias            : Immediate
+  imm             : Immediate
+  deriving BEq, FromCBOR, FromJson, FromSexp, Repr, ToCBOR, ToJson, ToSexp
+
+/- AffineSelect instruction
+
+Generates values using the `maskPattern` and runs them through `op`. If
+the comparison is true, the value from `in` is used, otherwise `fill_value` is used.
+out[k] = (mask[k] <op> 0) ? in[k]  : fill_value
+-/
+@[serde tag = 147]
+structure AffineSelect where
+  dst         : TensorRef
+  src         : TensorRef
+  fillMode    : AffineSelectCmp
+  fillReg     : Reg
+  maskPattern : DataPattern
+  deriving BEq, FromCBOR, FromJson, FromSexp, Repr, ToCBOR, ToJson, ToSexp
+
+/- DmaCopy instruction
+
+Generate descriptors to use the DMA to perform a copy.
+
+TODO: this operation is stateful since it uses the DMA queues. How
+do we represent that at the KLR level?
+-/
+@[serde tag = 148]
+structure DmaCopy where
+  dst            : TensorRef
+  src            : TensorRef
+  compute_op     : DgeComputeOp
+  dstBoundsCheck : DmaBounds
+  srcBoundsCheck : DmaBounds
+  deriving BEq, FromCBOR, FromJson, FromSexp, Repr, ToCBOR, ToJson, ToSexp
+
+/- DmaTranspose instruction
+Use the DMA to reverse the dimensions of a tensor.
+-/
+@[serde tag = 149]
+structure DmaTranspose where
+  dst : TensorRef
+  src : TensorRef
+  deriving BEq, FromCBOR, FromJson, FromSexp, Repr, ToCBOR, ToJson, ToSexp
+
+/- Transpose Instruction
+
+Uses the DVE engine to do a transpose on 32x32 tiles of tensors up to 4d.
+The total size of the accesses must be a multiple of 32x32, and the src and dest
+must be the same size. The number of partitions must be a multiple of 32.
+-/
+@[serde tag = 150]
+structure Transpose where
+  dst : TensorRef
+  src : TensorRef
+  deriving BEq, FromCBOR, FromJson, FromSexp, Repr, ToCBOR, ToJson, ToSexp
+
+/- LoadMaskRegister instruction
+
+Sets a register to be the MaskRegister in the DVE
+-/
+@[serde tag = 151]
+structure LoadMaskRegister where
+  regNum : Reg
+  deriving BEq, FromCBOR, FromJson, FromSexp, Repr, ToCBOR, ToJson, ToSexp
+
+/-
+Use the DVE to shuffle the data in src into dst based on MaskRegister
+-/
+@[serde tag = 152]
+structure Shuffle where
+  dst : TensorRef
+  src : TensorRef
+  deriving BEq, FromCBOR, FromJson, FromSexp, Repr, ToCBOR, ToJson, ToSexp
+
+/- MemSet instruction
+
+Sets `count` elements of `dst` to `value`
+-/
+@[serde tag = 153]
+structure MemSet where
+  dst   : TensorRef
+  value : UInt32
+  count : Nat
+  deriving BEq, FromCBOR, FromJson, FromSexp, Repr, ToCBOR, ToJson, ToSexp
+
+/- Iota Instruction
+Generates values using `pattern` and writes them to `dst` -/
+@[serde tag = 154]
+structure Iota where
+  dst : TensorRef
+  pattern : DataPattern
+  deriving BEq, FromCBOR, FromJson, FromSexp, Repr, ToCBOR, ToJson, ToSexp
+
+/- LoadStationary Instruction
+
+Loads a matrix into the PE.
+-/
+@[serde tag = 155]
+structure LoadStationary where
+  src         : TensorRef
+  isTranspose : Bool
+  deriving BEq, FromCBOR, FromJson, FromSexp, Repr, ToCBOR, ToJson, ToSexp
+
+/- MatMul instruction
+
+Performs a matmul against the currently loaded tensor using the PE -/
+@[serde tag = 156]
+structure MatMul where
+  dst                : TensorRef
+  moving             : TensorRef
+  psumAccumulateFlag : MatmulGroupElement
+  deriving BEq, FromCBOR, FromJson, FromSexp, Repr, ToCBOR, ToJson, ToSexp
+
+/- LocalGather instruction
+-/
+@[serde tag = 157]
+structure LocalGather where
+  dst               : TensorRef
+  src               : TensorRef
+  indexMissBehavior : IndexMissBehavior
+  /- Set to true when this is the last local gather operation in a group
+  to free the pool buffer -/
+  freePoolBuffer    : Bool
+  deriving BEq, FromCBOR, FromJson, FromSexp, Repr, ToCBOR, ToJson, ToSexp
+
+/- RangeSelect instruction
+-/
+@[serde tag = 158]
+structure RangeSelect where
+  dst            : TensorRef
+  src            : TensorRef
+  reduceCommand  : AccumCmd
+  reduceOp       : AluOp
+  base           : Float32
+  fillValue      : Float32
+  compOp0        : AluOp
+  compOp1        : AluOp
+  bound0         : Immediate
+  bound1         : Immediate
+  deriving BEq, FromCBOR, FromJson, FromSexp, Repr, ToCBOR, ToJson, ToSexp
+
+/- ScalarTensorTensor instruction
+
+```
+if accumulator_cmd == ZeroAccumulator:
+    accum_value = 0
+scalar_result = src0 op_0 imm0 # broadcast imm0 onto src0
+dst = scalar_result op_1 src1
+if (accumulator_cmd == ZeroAccumulator) or (accumulator_cmd == Accumulator):
+    accum_value += dst
+```
+-/
+@[serde tag = 159]
+structure ScalarTensorTensor where
+  dst             : TensorRef
+  src0            : TensorRef
+  src1            : TensorRef
+  op0             : AluOp
+  op1             : AluOp
+  reverseOperands : TensorScalarReverseOps
+  imm0            : Immediate
+  accumulatorCmd  : AccumCmd
+  deriving BEq, FromCBOR, FromJson, FromSexp, Repr, ToCBOR, ToJson, ToSexp
+
+/- CopyPredicated instruction
+
+Copies each element from src to dst for which predicate is not 0 -/
+@[serde tag = 160]
+structure CopyPredicated where
+  dst       : TensorRef
+  src       : TensorRef
+  predicate : TensorRef
+  deriving BEq, FromCBOR, FromJson, FromSexp, Repr, ToCBOR, ToJson, ToSexp
+
+/- TensorTensorScan instruction
+
+for lane_id in range(num_active_channels):
+    internal_state = imm0
+    for src0_elem, src1_elem in packed(src0_mem_pattern, src1_mem_pattern):
+        new_result = (src0_elem op0 internal_state) op1 src1_elem
+        internal_state = new_result
+        dst_mem_pattern.append(new_result)
+-/
+@[serde tag = 161]
+structure TensorTensorScan where
+  dst             : TensorRef
+  src0            : TensorRef
+  src1            : TensorRef
+  op0             : AluOp
+  op1             : AluOp
+  reverseOperands : TensorScalarReverseOps
+  imm0            : Immediate
+  accumulatorCmd  : AccumCmd
+  deriving BEq, FromCBOR, FromJson, FromSexp, Repr, ToCBOR, ToJson, ToSexp
+
+/- MatchValueLoad instruction
+
+Loads values into the DVE's MatchValue registers -/
+@[serde tag = 162]
+structure MatchValueLoad where
+  src : TensorRef
+  deriving BEq, FromCBOR, FromJson, FromSexp, Repr, ToCBOR, ToJson, ToSexp
+
+
+/- FindIndex8 instruction
+
+For each element in MatchValue register, find the first element of src that
+matches and stores its index in dst. -/
+@[serde tag = 163]
+structure FindIndex8 where
+  dst : TensorRef
+  src : TensorRef
+  deriving BEq, FromCBOR, FromJson, FromSexp, Repr, ToCBOR, ToJson, ToSexp
+
+/- MatchReplace8 instruction
+
+Same as FindIndex8, but replaces the found values in src with `replaceValue`-/
+@[serde tag = 164]
+structure MatchReplace8 where
+  dst          : TensorRef
+  src          : TensorRef
+  replaceValue : Float32
+  deriving BEq, FromCBOR, FromJson, FromSexp, Repr, ToCBOR, ToJson, ToSexp
+
+/- Max8 instruction
+
+Finds the 8 largest values in src and writes them to dst -/
+@[serde tag = 165]
+structure Max8 where
+  dst : TensorRef
+  src : TensorRef
+  deriving BEq, FromCBOR, FromJson, FromSexp, Repr, ToCBOR, ToJson, ToSexp
+
+/- BatchNormAggregate instruction
+-/
+@[serde tag = 166]
+structure BatchNormAggregate where
+  dst : TensorRef
+  src : TensorRef
+  deriving BEq, FromCBOR, FromJson, FromSexp, Repr, ToCBOR, ToJson, ToSexp
+
+/- BatchNormStats instruction
+-/
+@[serde tag = 167]
+structure BatchNormStats where
+  dst : TensorRef
+  src : TensorRef
+  deriving BEq, FromCBOR, FromJson, FromSexp, Repr, ToCBOR, ToJson, ToSexp
+
+/- Reciprocal instruction
+-/
+@[serde tag = 168]
+structure Reciprocal where
+  dst  : TensorRef
+  src  : TensorRef
+  deriving BEq, FromCBOR, FromJson, FromSexp, Repr, ToCBOR, ToJson, ToSexp
+
+/- Copy instruction
+Copy src to dst -/
+@[serde tag = 169]
+structure Copy where
+  dst   : TensorRef
+  src   : TensorRef
+  /- TODO: what is this for? -/
+  opDim : Option TensorSubDim
+  deriving BEq, FromCBOR, FromJson, FromSexp, Repr, ToCBOR, ToJson, ToSexp
+
+/- TensorReduce instruction
+
+Reduces a tensor along specified dimensions -/
+@[serde tag = 170]
+structure TensorReduce where
+  dst          : TensorRef
+  src          : TensorRef
+  op           : AluOp
+  opDim        : TensorSubDim
+  -- the negated field is only relevant for arithmetic operations
+  negated      : Bool
+  deriving BEq, FromCBOR, FromJson, FromSexp, Repr, ToCBOR, ToJson, ToSexp
+
+@[serde tag = 171]
 inductive Operator where
-  | load : Operator
-  | save : Operator
-  | memset : Nat -> Operator /- the Nat operand is uint32_t -/
-  | tensorScalar : TensorScalar -> Operator
-  | tensorScalarAddr : TensorScalarAddr -> Operator
-  deriving Repr, BEq
+  | Activate (op : Activate)
+  | AffineSelect (op : AffineSelect)
+  | BatchNormAggregate (op : BatchNormAggregate)
+  | BatchNormStats (op : BatchNormStats)
+  | Copy (op : Copy)
+  | CopyPredicated (op : CopyPredicated)
+  | DmaCopy (op : DmaCopy)
+  | DmaTranspose (op : DmaTranspose)
+  | Dropout (op : Dropout)
+  | FindIndex8 (op : FindIndex8)
+  | Iota (op : Iota)
+  | LoadMaskRegister (op : LoadMaskRegister)
+  | LoadStationary (op : LoadStationary)
+  | LocalGather (op : LocalGather)
+  | MatMul (op : MatMul)
+  | MatchReplace8 (op : MatchReplace8)
+  | MatchValueLoad (op : MatchValueLoad)
+  | Max8 (op : Max8)
+  | MemSet (op : MemSet)
+  | RangeSelect (op : RangeSelect)
+  | Reciprocal (op : Reciprocal)
+  | ScalarTensorTensor (op : ScalarTensorTensor)
+  | Shuffle (op : Shuffle)
+  | TensorReduce (op : TensorReduce)
+  | TensorTensorScan (op : TensorTensorScan)
+  | Transpose (op : Transpose)
+  deriving BEq, FromCBOR, FromJson, FromSexp, Repr, ToCBOR, ToJson, ToSexp
