KLR/Core/Tensor.lean
@@ -1,0 +1,469 @@
+/-
+Copyright (c) 2024 Amazon.com, Inc. or its affiliates. All Rights Reserved.
+Released under Apache 2.0 license as described in the file LICENSE.
+Authors: Paul Biberstein, Paul Govereau, Pavel Potapov, Sean McLaughlin, Markus De Medeiros
+-/
+import KLR.Serde.Attr
+import KLR.Serde.Elab
+import KLR.Util
+
+/-!
+# Definitions for Tensor representations
+-/
+namespace KLR.Core
+open Lean (FromJson ToJson)
+open Serde (FromCBOR ToCBOR)
+open Util (FromSexp ToSexp)
+
+-- Memory types on hardware
+@[serde tag = 110]
+inductive Memory where
+  | hbm | sbuf | pmem | reg
+  deriving BEq, FromCBOR, FromJson, FromSexp, Repr, ToCBOR, ToJson, ToSexp
+
+/-
+Tensor element types supported by hardware.
+
+The HW always performs operations on 32-bit types. However, when reading from
+or writing to memory, automatic conversion to and from the following types is
+supported.
+-/
+@[serde tag = 111]
+inductive Dtype where
+  | bfloat16
+  | float8e3 | float8e4 | float8e5
+  | float16 | float32 | float32r
+  | int8 | int16 | int64 | int32
+  | uint8 | uint16 | uint32 | uint64
+  with
+    @[computed_field]
+    size : Dtype -> Nat
+    | .uint8 | .int8 | .float8e3 | .float8e4 | .float8e5 => 1
+    | .uint16 | .int16 | .bfloat16 | .float16 => 2
+    | .uint32 | .int32 | .float32 | .float32r => 4
+    | .uint64 | .int64 => 8
+    @[computed_field]
+    isInt : Dtype -> Bool
+    | .int8 | .int16 | .int64 | .int32
+    | .uint8 | .uint16 | .uint32 | .uint64 => true
+    | _ => false
+  deriving BEq, FromCBOR, FromJson, FromSexp, Repr, ToCBOR, ToJson, ToSexp
+
+/-
+A tensor shape is a list of the sizes of each dimension of the tensor. By
+convention, the first dimension is always the "partition" dimension, and the
+remaining dimensions are "free" dimensions. When laid out in memory, the
+partition dimension will correspond to the memory partition.
+-/
+@[serde tag = 112]
+structure Shape where
+  parDim : Nat
+  freeDims : List Nat
+  deriving BEq, FromCBOR, FromJson, FromSexp, Repr, ToCBOR, ToJson, ToSexp
+
+namespace Shape
+
+def toList (shape : Shape) : List Nat :=
+  shape.parDim :: shape.freeDims
+
+def fromList : List Nat -> Err Shape
+  | [] => throw "invalid shape"
+  | p :: f => return ⟨ p, f ⟩
+
+def freeElements (shape : Shape) : Nat :=
+  shape.freeDims.foldl (. * .) 1
+
+instance : Inhabited Shape where
+  default := { parDim := 0, freeDims := [] }
+
+instance : ToString Shape where
+  toString shape := toString shape.toList
+
+end Shape
+
+/-
+An Address represents a region of memory. Each address has a memory type, and
+the starting location and size of the memory region. The memory regions are
+always two-dimensional and the start and size are expressed in bytes. The
+starting location can be omitted to have the compiler choose this for you.
+
+The Address structure is represented as a "pointer" term during tracing.
+-/
+@[serde tag = 113]
+structure Address where
+  memory : Memory
+  parSize : Nat
+  freeSize : Nat
+  parOffset : Option Nat := none
+  freeOffset : Option Nat := none
+  deriving BEq, FromCBOR, FromJson, FromSexp, Repr, ToCBOR, ToJson, ToSexp
+
+namespace Address
+
+def defaultSize (shape : Shape) (dtype : Dtype) : (Nat × Nat) :=
+  (shape.parDim, shape.freeElements * dtype.size)
+
+def withDefaultSize (addr : Address) (shape : Shape) (dtype : Dtype) : Address :=
+  let (p, f) := defaultSize shape dtype
+  { addr with parSize := p, freeSize := f }
+
+instance : Inhabited Address where
+  default := {
+    memory := .sbuf
+    parSize := 0
+    freeSize := 0
+  }
+
+end Address
+
+/--
+TensorSram represents a tensor in SRam (either SBuf of PSum) at runtime. Each
+runtime tensor has a dtype, shape, and address. The address size must be large
+enough to hold the tensor. Unlike a TensorView, a TensorSram may not yet have
+an address assigned, or it may be spilled by the allocator and need to be
+reloaded. If a TensorSram has a complete Address, it can be converted to a
+TensorView, if there is enough space in the SBuf (or PSum).
+-/
+@[serde tag = 114]
+structure TensorSram where
+  name    : String
+  dtype   : Dtype
+  shape   : Shape
+  address : Address
+  parWF   : shape.parDim <= address.parSize
+  freeWF  : shape.freeElements * dtype.size <= address.freeSize
+  deriving Repr
+
+instance : BEq TensorSram where
+  beq l r := l.name == r.name &&
+             l.dtype == r.dtype &&
+             l.shape == r.shape &&
+             l.address == r.address
+-- TODO
+instance : FromCBOR TensorSram := ⟨ fun _ => throw "" ⟩
+instance : FromJson TensorSram := ⟨ fun _ => throw "" ⟩
+instance : FromSexp TensorSram := ⟨ fun _ => throw "" ⟩
+instance : ToCBOR TensorSram := ⟨ fun _ => default ⟩
+instance : ToSexp TensorSram := ⟨ fun _ => default ⟩
+instance : ToJson TensorSram := ⟨ fun _ => default ⟩
+
+namespace TensorSram
+
+-- TODO: should .mk be private?
+def make (name : String)
+         (dtype : Dtype)
+         (shape : Shape)
+         (addr : Option Address) : Err TensorSram := do
+  let addr := addr.getD (Address.withDefaultSize default shape dtype)
+  if parWF : shape.parDim <= addr.parSize then
+    if freeWF : shape.freeElements * dtype.size <= addr.freeSize then
+      return ⟨ name, dtype, shape, addr, parWF, freeWF ⟩
+  throw "Tensor does not fit within memory location"
+
+def withShape (name : TensorSram) (shape : Shape) : Err TensorSram :=
+  make name.name name.dtype shape (name.address.withDefaultSize shape name.dtype)
+
+end TensorSram
+
+/--
+Basic indexing elements: integers and slices.
+These are used for basic indexing, such as:
+  t[1, 2]
+  t[0:10, :]
+  t[5, 0:10:2]
+
+The tracing process will generate Indexes relative to a given shape,
+and therefore we do not have `None` or `...` as possibilities.
+-/
+@[serde tag = 115]
+structure Slice where
+  l : Nat
+  u : Nat
+  step : Int
+  wf : step ≠ 0
+  --deriving BEq, FromCBOR, FromJson, FromSexp, Repr, ToCBOR, ToJson, ToSexp
+  deriving BEq, Repr
+
+-- TODO
+instance : FromCBOR Slice := ⟨ fun _ => throw "" ⟩
+instance : FromJson Slice := ⟨ fun _ => throw "" ⟩
+instance : FromSexp Slice := ⟨ fun _ => throw "" ⟩
+instance : ToCBOR Slice := ⟨ fun _ => default ⟩
+instance : ToSexp Slice := ⟨ fun _ => default ⟩
+instance : ToJson Slice := ⟨ fun _ => default ⟩
+
+namespace Slice
+
+def make (l u : Nat) (step : Int) : Err Slice := do
+  if wf : step ≠ 0 then
+    return Slice.mk l u step wf
+  throw "Step size cannot be 0"
+
+instance : Inhabited Slice where
+  default := Slice.mk 0 1 1 Int.one_ne_zero
+
+def make! (l u : Nat) (step : Int) : Slice := get! $  make l u step
+
+def size (slice : Slice) : Nat :=
+  let step := slice.step
+    if step < 0 then (slice.l - slice.u) / step.natAbs
+    else natDivCeil (slice.u - slice.l) step.toNat
+
+#guard (make! 0 10 1).size == 10
+#guard (make! 10 0 (-1)).size == 10
+#guard (make! 0 10 (-1)).size == 0
+#guard (make! 10 0 1).size == 0
+
+end Slice
+
+@[serde tag = 116]
+inductive Index where
+  | coord (e : Nat)
+  | slice (slice : Slice)
+  deriving BEq, FromCBOR, FromJson, FromSexp, Repr, ToCBOR, ToJson, ToSexp
+
+-- Compute the number of elements an index represents
+def Index.size : Index -> Nat
+ | .coord _ => 1
+ | .slice s => s.size
+
+/--
+Complete Basic Indexing expression
+
+The number of indexes must match the dimension of the tensor.
+-/
+
+@[serde tag = 117]
+structure AccessBasic where
+  tensor : TensorSram
+  indexes : List Index
+  lenWF : tensor.shape.freeDims.length + 1 = indexes.length
+  deriving Repr
+
+instance : BEq AccessBasic where
+  beq l r := l.tensor == r.tensor && l.indexes == r.indexes
+
+-- TODO
+instance : FromCBOR AccessBasic := ⟨ fun _ => throw "" ⟩
+instance : FromJson AccessBasic := ⟨ fun _ => throw "" ⟩
+instance : FromSexp AccessBasic := ⟨ fun _ => throw "" ⟩
+instance : ToCBOR AccessBasic := ⟨ fun _ => default ⟩
+instance : ToSexp AccessBasic := ⟨ fun _ => default ⟩
+instance : ToJson AccessBasic := ⟨ fun _ => default ⟩
+
+namespace AccessBasic
+
+def make (t : TensorSram) (i : List Index) : Err AccessBasic := do
+  if lenWF : t.shape.freeDims.length + 1 = i.length then
+    return ⟨ t, i, lenWF ⟩
+  throw "invalid basic access"
+
+def shape (a : AccessBasic) : Err Shape :=
+  if let p::l := a.indexes then
+    .ok ⟨ p.size, l.map Index.size ⟩
+  else .error "invalid access"
+
+def shape! (a : AccessBasic) : Shape := get! (shape a)
+
+theorem shape.noFail :
+  forall (a : AccessBasic), AccessBasic.shape a ≠ Except.error s := by
+  intro a
+  unfold AccessBasic.shape
+  let { tensor, indexes, lenWF : AccessBasic } := a
+  induction indexes <;> simp ; trivial
+  done
+
+end AccessBasic
+
+/--
+Access pattern elements.
+
+These are used for HW-native indexing which consists of an offset and a list of
+access pattern pairs. Each pair specifies a step size and the number of steps
+to take. The first changes the slowest, and the last pair changes the fastest.
+For example, in the list of pairs:
+
+  [ (3,2), (1,3) ]
+
+the first pair will produce the values 0,3 and the second pair will produce the
+values 0,1,2. Added together, the pairs produce the values:
+
+  0, 1, 2, 3, 4, 5.
+
+which is equivalent to the basic index [0:2,0:3] for a standard tensor layout.
+-/
+@[serde tag = 118]
+structure APPair where
+  step : Int := 1
+  num : Nat := 1
+  deriving BEq, FromCBOR, FromJson, FromSexp, Repr, ToCBOR, ToJson, ToSexp
+
+/--
+Complete access patterns
+
+A complete access pattern has a list of APPairs, a number of partitions, and an
+offset. In NKI, the first access pattern pair corresponds to the partition
+dimension, and the step size of this first pair must be one. So, in the
+complete access pattern, we only store the `num` field of the first pair. The
+offset field allows for an arbitrary offset to be applied to each partition.
+
+Put together, a complete access pattern would be written as:
+
+  t[[ offset, (1, parNum), (step1,num1), (step2,num2), ... ]]
+
+With a meaning of:
+
+  forall p < parNum, x < num1, y < num2, ...
+    offset + p + x * step1 + y * step2 + ...
+
+The elements generated above are multiplied by the dtype size of the tensor to
+get the final memory addresses.
+-/
+
+@[serde tag = 119]
+structure AccessPattern where
+  tensor : TensorSram
+  parNum : Nat
+  freePattern : List APPair
+  offset : Nat := 0
+  deriving BEq, FromCBOR, FromJson, FromSexp, Repr, ToCBOR, ToJson, ToSexp
+
+namespace AccessPattern
+
+def shape (ap : AccessPattern) : Shape :=
+  .mk ap.parNum $ ap.freePattern.map fun pair => pair.num
+
+-- Partitions are not counted in bytes or elements; I'll call them logical "rows".
+def partitionRowOffset (ap : AccessPattern) : Nat :=
+  ap.tensor.address.parOffset.getD 0
+
+def freeByteOffset (ap : AccessPattern) : Nat :=
+  ap.tensor.address.freeOffset.getD 0 + ap.offset
+
+-- We can't find documentation that the free offset must be aligned by dtype size, but we think
+-- it's probably the case. It certainly makes calculating indexes easier so we're going with it
+-- for now.
+def freeElementOffset (ap : AccessPattern) : Nat :=
+  ap.freeByteOffset / ap.tensor.dtype.size
+
+end AccessPattern
+
+-- Tensor access: whole tensor (simple), basic indexing, or access pattern
+-- TODO: add advanced indexing (tensor indirect) inductive Access where
+
+@[serde tag = 120]
+inductive Access where
+  | simple  (tensor : TensorSram) : Access
+  | basic   (access : AccessBasic) : Access
+  | pattern (access : AccessPattern) : Access
+  deriving BEq, FromCBOR, FromJson, FromSexp, Repr, ToCBOR, ToJson, ToSexp
+
+namespace Access
+
+def mkBasic (t : TensorSram) (i : List Index) : Err Access :=
+  return .basic (<- AccessBasic.make t i)
+
+def tensor : Access -> TensorSram
+  | simple tensor
+  | basic {tensor, ..}
+  | pattern {tensor, ..} => tensor
+
+def shape : Access -> Err Shape
+  | .simple t => return t.shape
+  | .basic b => b.shape
+  | .pattern ap => return ap.shape
+
+theorem shape.noFail :
+  forall (a : Access), Access.shape a ≠ Except.error s := by
+  unfold Access.shape pure
+  unfold Applicative.toPure
+  unfold Monad.toApplicative
+  unfold Except.instMonad Except.pure
+  intro a
+  induction a <;> simp
+  apply AccessBasic.shape.noFail
+  done
+
+-- We could make a pure variant of shape, but proofs about this
+-- function may be difficult due to the dependent matching
+def shapePure (a : Access) : Shape :=
+  match m:a.shape with
+  | .ok x => x
+  | .error _ =>
+     have h : False := by apply (shape.noFail a); trivial
+     nomatch h
+
+end Access
+
+/-
+A tensor in HBM. The address is an offset into HBM.
+-/
+@[serde tag = 121]
+structure TensorHbm where
+  dtype   : Dtype
+  address : Nat
+  shape   : List Nat
+  strides : List Nat
+  deriving BEq, FromCBOR, FromJson, FromSexp, Repr, ToCBOR, ToJson, ToSexp
+
+-- register number
+abbrev Reg := Nat
+
+@[serde tag = 122]
+inductive ParQuadrant where
+  | par0 | par32 | par64 | par96
+  deriving BEq, FromCBOR, FromJson, FromSexp, Repr, ToCBOR, ToJson, ToSexp
+
+/-
+A structure representing the layout of a tensor in SRam. This maps very closely
+to the way that the ISA expects tensor accesses to be expressed. Specifically,
+it separates the parallel dimension from the rest of the dimensions and
+includes constraints like the fact that the parallel dimension stride is always 1.
+
+              0┌──────────────────────┐
+               │                      │
+             32│                      │
+               │                      │
+             64│                      │
+               │                      │
+parQuadrant─►96│    ┌───────┐│        │
+               │    └───────┘│parSize │
+               └──────────────────────┘
+                    ▲
+                    │
+               parOffset
+-/
+@[serde tag = 123]
+structure TensorView where
+  name    : String
+  dtype   : Dtype
+  -- Which parallel dimension channel this tensor starts at
+  parQuadrant : ParQuadrant
+  -- The size of this tensor in the parallel dimension
+  parDim : Nat
+  -- The offset in the partition channel of this tensor
+  freeOffset : Nat := 0
+  -- The length and stride of each dimension besides the first
+  freePattern: List APPair
+  deriving BEq, FromCBOR, FromJson, FromSexp, Repr, ToCBOR, ToJson, ToSexp
+
+/-
+The type that is passed to instructions to refer to a tensor in SBUF. We abstract
+over whether the tensor is a literal or stored in a shape register.
+-/
+@[serde tag = 124]
+inductive TensorRef where
+  | abstract (access : Access)
+  | literal (view : TensorView)
+  | register (reg : Reg)
+  deriving BEq, FromCBOR, FromJson, FromSexp, Repr, ToCBOR, ToJson, ToSexp
+
+/-
+This type reprents tensor arguments that can be passed to kernel function.
+Tensor arguments can be either HBM or abstract SRAM tensors.
+-/
+@[serde tag = 125]
+inductive TensorArg where
+  | hbm (tensor : TensorHbm)
+  | sram (tensor : TensorSram)
+  deriving BEq, FromCBOR, FromJson, FromSexp, Repr, ToCBOR, ToJson, ToSexp
